uniformize UntypedSemantics

coq/UntypedSemantics.v
@@ -1,7 +1,6 @@
 (*! Language | Semantics of typed Kôika programs !*)
-Require Export Koika.Common Koika.Environments Koika.ULogs Koika.Syntax
-        Koika.Syntax.
-
+Require Export Koika.Common Koika.Environments Koika.Syntax Koika.UntypedLogs.
+Import PrimTyped PrimUntyped.
 
 Ltac destr_in H :=
   match type of H with
@@ -10,11 +9,10 @@ Ltac destr_in H :=
 
 Ltac destr :=
   match goal with
-    |- context[match ?a with _ => _ end] => destruct a eqn:?; try congruence
+  |- context[match ?a with _ => _ end] => destruct a eqn:?; try congruence
   end.
 
-Ltac inv H :=
-  inversion H; try subst; clear H.
+Ltac inv H := inversion H; try subst; clear H.
 
 Section Interp.
   Context {pos_t var_t fn_name_t reg_t ext_fn_t: Type}.
@@ -31,29 +29,26 @@ Section Interp.
   Context {REnv: Env reg_t}.
 
   Notation Log := (@_ULog val reg_t REnv).
-
-  (* Notation rule := (rule pos_t var_t fn_name_t R Sigma). *)
   Notation uaction := (uaction pos_t var_t fn_name_t reg_t ext_fn_t).
-  (* Notation scheduler := (scheduler pos_t rule_name_t). *)
 
-  Definition tcontext (sig: tsig var_t) :=
-    context (fun k_tau => val) sig.
+  Definition tcontext (sig: tsig var_t) := context (fun k_tau => val) sig.
 
   Definition acontext (sig argspec: tsig var_t) :=
     context (fun k_tau => uaction) argspec.
 
   Section Action.
-
     Fixpoint ucassoc {sig: tsig var_t} (Gamma: tcontext sig) (k: var_t)
       : option val
-      :=
-        match Gamma with
-        | CtxEmpty => None
-        | CtxCons k' v Gamma => if eq_dec k (fst k') then Some v else ucassoc Gamma k
-        end.
+    :=
+      match Gamma with
+      | CtxEmpty => None
+      | CtxCons k' v Gamma =>
+        if eq_dec k (fst k') then Some v else ucassoc Gamma k
+      end.
 
     Lemma cassoc_ucassoc:
-      forall (sig: tsig var_t) (ND: NoDup (map fst sig)) (Gamma: tcontext sig) k,
+      forall (sig: tsig var_t) (ND: NoDup (map fst sig)) (Gamma: tcontext sig)
+        k,
       forall (m: member k sig), ucassoc Gamma (fst k) = Some (cassoc m Gamma).
     Proof.
       induction Gamma. simpl. intros.
@@ -61,32 +56,28 @@ Section Interp.
       intros. simpl. destruct eq_dec.
       destruct k, k0; simpl in *. subst.
       inversion m; subst.
-      generalize (
-          fun nd => member_NoDup (v0, t) (EqDec_pair _ _) nd m (MemberHd _ _)
-        ).
+      generalize
+        (fun nd => member_NoDup (v0, t) (EqDec_pair _ _) nd m (MemberHd _ _)).
       intros. rewrite H. simpl. auto. apply NoDup_map_inv with (f:= fst).
       simpl; auto.
       apply member_In in X. inversion ND. subst. exfalso; apply H1.
       apply in_map_iff. eexists; split. 2: apply X. reflexivity.
       inversion m. subst. congruence. subst.
-      generalize (fun nd => member_NoDup k0 (EqDec_pair _ _)
-                                         nd m (MemberTl _ _ _ X)).
+      generalize
+        (fun nd => member_NoDup k0 (EqDec_pair _ _) nd m (MemberTl _ _ _ X)).
       intros. rewrite H. simpl. eapply IHGamma. simpl in ND; inversion ND; auto.
       apply NoDup_map_inv with (f:= fst). simpl; auto.
     Qed.
 
     Fixpoint val_of_value {tau: type} (x: type_denote tau) {struct tau} : val :=
-      let val_of_struct_value :=
-          (fix val_of_struct_value
-               {fields}
-               (x: struct_denote fields)
-           : list val :=
-             match fields return struct_denote fields -> list val with
-             | [] => fun _ => []
-             | (nm, tau) :: fields =>
-               fun '(x, xs) =>
-                 val_of_value x :: (val_of_struct_value xs)
-             end x) in
+      let val_of_struct_value := (
+        fix val_of_struct_value {fields} (x: struct_denote fields) : list val :=
+          match fields return struct_denote fields -> list val with
+          | [] => fun _ => []
+          | (nm, tau) :: fields =>
+            fun '(x, xs) =>
+              val_of_value x :: (val_of_struct_value xs)
+          end x) in
       match tau return type_denote tau -> val with
       | bits_t sz => fun bs => Bits sz  (vect_to_list bs)
       | enum_t sig => fun bs => Enum sig (vect_to_list bs)
@@ -104,8 +95,7 @@ Section Interp.
 
     Lemma ubits_of_value_len:
       forall {tau} (v: type_denote tau) bs,
-        ubits_of_value (val_of_value v) = bs ->
-        List.length bs = type_sz tau.
+      ubits_of_value (val_of_value v) = bs -> List.length bs = type_sz tau.
     Proof.
       fix IHt 1. destruct tau; simpl; intros; subst.
       apply vect_to_list_length.
@@ -130,8 +120,8 @@ Section Interp.
 
     Lemma ubits_of_value_ok:
       forall {tau} (v: type_denote tau) bs,
-        ubits_of_value (val_of_value v) = bs ->
-        vect_to_list (bits_of_value v) = bs.
+      ubits_of_value (val_of_value v) = bs ->
+      vect_to_list (bits_of_value v) = bs.
     Proof.
       fix IHt 1. destruct tau; simpl; intros; subst; auto.
       - revert sig v. destruct sig. simpl.
@@ -154,14 +144,14 @@ Section Interp.
 
     Fixpoint replace {sig: tsig var_t} k (v: val) (Gamma: tcontext sig)
       : tcontext sig
-      :=
-        match Gamma with
-        | CtxEmpty => CtxEmpty
-        | CtxCons k0 v0 Gamma =>
-          if eq_dec k (fst k0)
-          then CtxCons k0 v Gamma
-          else CtxCons k0 v0 (replace k v Gamma)
-        end.
+    :=
+      match Gamma with
+      | CtxEmpty => CtxEmpty
+      | CtxCons k0 v0 Gamma =>
+        if eq_dec k (fst k0)
+        then CtxCons k0 v Gamma
+        else CtxCons k0 v0 (replace k v Gamma)
+      end.
 
     Definition bits_split (n: nat) {sz} (v: bits sz)
       : option (bits n * bits (sz - n)).
@@ -172,12 +162,14 @@ Section Interp.
       exact (Some (v0, v1)).
     Defined.
 
-    Fixpoint take_drop {A: Type} (n: nat) (l: list A) : option (list A * list A) :=
+    Fixpoint take_drop {A: Type} (n: nat) (l: list A)
+      : option (list A * list A)
+    :=
       match n with
-        O => Some ([], l)
+      | O => Some ([], l)
       | S n =>
         match l with
-          [] => None
+        | [] => None
         | a::l =>
           let/opt2 l1, l2 := take_drop n l in
           Some (a::l1, l2)
@@ -186,25 +178,24 @@ Section Interp.
 
     Definition take_drop' {A: Type} n (l: list A) :=
       match take_drop n l with
-        None => (l,[])
+      | None => (l,[])
       | Some (l1, l2) => (l1, l2)
       end.
 
     Fixpoint bits_splitn (nb sz_elt: nat) (bs: list bool)
       : option (list (list bool))
-      :=
-        match nb with
-          O => Some []
-        | S nb =>
-          let/opt2 hd, rest := take_drop sz_elt bs in
-          let/opt tl := bits_splitn nb sz_elt rest in
-          Some (hd :: tl)
-        end.
+    :=
+      match nb with
+      | O => Some []
+      | S nb =>
+        let/opt2 hd, rest := take_drop sz_elt bs in
+        let/opt tl := bits_splitn nb sz_elt rest in
+        Some (hd :: tl)
+      end.
 
     Lemma take_drop_succeeds:
       forall {A:Type} (n: nat) (l: list A) (LT: n <= Datatypes.length l),
-      exists la lb,
-        take_drop n l = Some (la, lb).
+      exists la lb, take_drop n l = Some (la, lb).
     Proof.
       induction n; simpl; intros; eauto.
       destruct l; simpl in LT. lia.
@@ -215,8 +206,8 @@ Section Interp.
 
     Lemma take_drop_spec:
       forall {A:Type} (n: nat) (l la lb: list A),
-        take_drop n l = Some (la, lb) ->
-        l = la ++ lb /\ List.length la = n /\ List.length lb = List.length l - n.
+      take_drop n l = Some (la, lb) ->
+      l = la ++ lb /\ List.length la = n /\ List.length lb = List.length l - n.
     Proof.
       induction n; simpl; intros; eauto.
       inversion H; clear H; subst. repeat split; try reflexivity. lia.
@@ -239,12 +230,14 @@ Section Interp.
 
     Lemma take_drop'_spec:
       forall {A:Type} (n: nat) (l la lb: list A),
-        take_drop' n l = (la, lb) ->
-        l = la ++ lb /\ List.length la <= n /\ List.length lb = List.length l - List.length la.
+      take_drop' n l = (la, lb) ->
+      l = la ++ lb /\ List.length la <= n /\
+        List.length lb = List.length l - List.length la.
     Proof.
       induction n; simpl; intros; eauto.
       inversion H; clear H; subst. repeat split; try reflexivity. simpl; lia.
-      destruct l; simpl in *. unfold take_drop' in H. simpl in *. inversion H; clear H.
+      destruct l; simpl in *. unfold take_drop' in H. simpl in *.
+      inversion H; clear H.
       simpl. repeat split; lia.
       destruct (take_drop' n l) as (l1 & l2) eqn:?.
       erewrite take_drop'_cons in H; eauto. inversion H; subst. simpl.
@@ -252,12 +245,9 @@ Section Interp.
       repeat split; auto. lia.
     Qed.
 
-
     Lemma app_eq_inv:
       forall {A:Type} (a b c d: list A),
-        a ++ b = c ++ d ->
-        List.length a = List.length c ->
-        a = c /\ b = d.
+      a ++ b = c ++ d -> List.length a = List.length c -> a = c /\ b = d.
     Proof.
       induction a; simpl; intros; eauto.
       - destruct c; simpl in H0; try congruence.
@@ -269,18 +259,15 @@ Section Interp.
 
     Inductive wt_val: type -> val -> Prop :=
     | wt_bits: forall n bs,
-        List.length bs = n ->
-        wt_val (bits_t n) (Bits n bs)
+      List.length bs = n -> wt_val (bits_t n) (Bits n bs)
     | wt_enum: forall sig bs,
-        List.length bs = enum_bitsize sig ->
-        wt_val (enum_t sig) (Enum sig bs)
+      List.length bs = enum_bitsize sig -> wt_val (enum_t sig) (Enum sig bs)
     | wt_struct: forall sig lv,
-        Forall2 (fun nt v => wt_val nt v) (map snd (struct_fields sig)) lv ->
-        wt_val (struct_t sig) (Struct sig lv)
+      Forall2 (fun nt v => wt_val nt v) (map snd (struct_fields sig)) lv ->
+      wt_val (struct_t sig) (Struct sig lv)
     | wt_array: forall sig lv,
-        Forall (fun v => wt_val (array_type sig) v) lv ->
-        List.length lv = array_len sig ->
-        wt_val (array_t sig) (Array sig lv).
+      Forall (fun v => wt_val (array_type sig) v) lv ->
+      List.length lv = array_len sig -> wt_val (array_t sig) (Array sig lv).
 
     Fixpoint size_type (t: type) :=
       match t with
@@ -293,43 +280,49 @@ Section Interp.
       end.
 
     Lemma wt_val_ind':
-      forall (P : type -> val -> Prop)
-             (Hbits: forall (n : nat) (bs : list bool), Datatypes.length bs = n -> P (bits_t n) (Bits n bs))
-             (Henum: forall (sig : enum_sig) (bs : list bool),
-                 Datatypes.length bs = enum_bitsize sig -> P (enum_t sig) (Enum sig bs))
-             (Hstruct: forall (sig : struct_sig) (lv : list val),
-                 Forall2 (fun (nt : type) (v : val) => wt_val nt v) (map snd (struct_fields sig)) lv ->
-                 Forall2 (fun (nt : type) (v : val) => wt_val nt v -> P nt v) (map snd (struct_fields sig)) lv ->
-                 P (struct_t sig) (Struct sig lv))
-             (Harray: forall (sig : array_sig) (lv : list val),
-                 Forall (fun v : val => wt_val (array_type sig) v) lv ->
-                 Forall (fun v : val => wt_val (array_type sig) v -> P (array_type sig) v) lv ->
-                 Datatypes.length lv = array_len sig -> P (array_t sig) (Array sig lv)),
-      forall (t : type) (v : val), wt_val t v -> P t v.
+      forall
+        (P : type -> val -> Prop)
+        (Hbits: forall (n : nat) (bs : list bool),
+          Datatypes.length bs = n -> P (bits_t n) (Bits n bs)
+        )
+        (Henum: forall (sig : enum_sig) (bs : list bool),
+          Datatypes.length bs = enum_bitsize sig -> P (enum_t sig) (Enum sig bs)
+        )
+        (Hstruct: forall (sig : struct_sig) (lv : list val),
+          Forall2 (fun (nt : type) (v : val) => wt_val nt v)
+            (map snd (struct_fields sig)) lv ->
+            Forall2 (fun (nt : type) (v : val) => wt_val nt v -> P nt v)
+              (map snd (struct_fields sig)) lv ->
+              P (struct_t sig) (Struct sig lv))
+        (Harray: forall (sig : array_sig) (lv : list val),
+          Forall (fun v : val => wt_val (array_type sig) v) lv ->
+          Forall (fun v : val => wt_val (array_type sig) v ->
+            P (array_type sig) v) lv ->
+              Datatypes.length lv = array_len sig ->
+                P (array_t sig) (Array sig lv)
+        ),
+        forall (t : type) (v : val), wt_val t v -> P t v.
     Proof.
       intros P Hbits Henum Hstruct Harray t v.
       remember (size_type t).
       revert t v Heqn.
       pattern n.
       eapply Nat.strong_right_induction with (z:=0).
-      {
-        red. red. intros. subst. tauto.
-      } 2: lia.
+      { red. red. intros. subst. tauto. }
+      2: lia.
       intros n0 _ Plt t t0 a Heqn.
-      assert (Plt':
-                forall t v,
-                  size_type t < n0 -> wt_val t v -> P t v
-             ).
-      {
-        intros. eapply Plt. 3: reflexivity. lia. auto. auto.
-      } clear Plt.
-      rename Plt' into Plt.
+      assert (Plt': forall t v, size_type t < n0 -> wt_val t v -> P t v).
+      { intros. eapply Plt. 3: reflexivity. lia. auto. auto. }
+      clear Plt.  rename Plt' into Plt.
       subst.
       inversion Heqn; subst; eauto.
       - eapply Hstruct. eauto.
         revert H.
         simpl in Plt.
-        assert (Forall (fun '(n,t) => forall v, wt_val t v -> P t v) (struct_fields sig)).
+        assert (
+          Forall (fun '(n,t) => forall v, wt_val t v -> P t v)
+          (struct_fields sig)
+        ).
         {
           revert Plt; clear. destruct sig. simpl.
           induction struct_fields; simpl; intros. constructor.
@@ -356,11 +349,9 @@ Section Interp.
       | Array sig lv => 1 + list_sum (map size_val lv)
       end.
 
-
-
     Lemma take_drop_succeeds_eq:
       forall {A:Type} (n: nat) (l: list A) (LT: n = Datatypes.length l),
-        take_drop n l = Some (l, []).
+      take_drop n l = Some (l, []).
     Proof.
       induction n; simpl; intros; eauto.
       destruct l; simpl in LT. reflexivity. lia.
@@ -370,8 +361,7 @@ Section Interp.
 
     Lemma take_drop_head:
       forall {A} n (l1 l2: list A),
-        n = List.length l1 ->
-        take_drop n (l1 ++ l2) = Some (l1, l2).
+      n = List.length l1 -> take_drop n (l1 ++ l2) = Some (l1, l2).
     Proof.
       intros. subst. revert l2.
       induction l1; simpl; intros; subst; eauto.
@@ -380,8 +370,8 @@ Section Interp.
 
     Lemma length_concat_same:
       forall {A} (l: list (list A)) sz,
-        Forall (fun x => List.length x = sz) l ->
-        Datatypes.length (List.concat l) = List.length l * sz.
+      Forall (fun x => List.length x = sz) l ->
+      Datatypes.length (List.concat l) = List.length l * sz.
     Proof.
       induction 1; simpl; intros; eauto.
       rewrite app_length; rewrite IHForall. lia.
@@ -390,8 +380,7 @@ Section Interp.
 
     Lemma ubits_of_value_len':
       forall tau v,
-        wt_val tau v ->
-        List.length (ubits_of_value v) = type_sz tau.
+      wt_val tau v -> List.length (ubits_of_value v) = type_sz tau.
     Proof.
       intros tau v WT.
       pattern tau, v.
@@ -414,9 +403,8 @@ Section Interp.
 
     Lemma bits_splitn_concat:
       forall sz l n,
-        Forall (fun l => List.length l = sz) l ->
-        List.length l = n ->
-        bits_splitn n sz (List.concat l) = Some l.
+      Forall (fun l => List.length l = sz) l ->
+      List.length l = n -> bits_splitn n sz (List.concat l) = Some l.
     Proof.
       intros. subst.
       induction H; simpl; intros; auto.
@@ -424,32 +412,31 @@ Section Interp.
       rewrite IHForall. simpl. reflexivity.
     Qed.
 
-
-    Fixpoint uvalue_of_bits {tau: type} (bs: list bool) {struct tau}: option val :=
-      let uvalue_of_struct_bits :=
-          (fix uvalue_of_struct_bits
-               {fields: list (string * type)}
-               (bs: list bool)
-           : option (list val) :=
-             match fields with
-             | [] => Some []
-             | (nm, tau) :: fields =>
-               let/opt2 b0, b1 := take_drop (List.length bs - type_sz tau) bs in
-               let/opt tl := uvalue_of_struct_bits (fields:=fields) b0 in
-               let/opt hd := uvalue_of_bits (tau:=tau) b1 in
-               Some ( hd :: tl)
-             end) in
+    Fixpoint uvalue_of_bits {tau: type} (bs: list bool) {struct tau}
+      : option val
+    :=
+      let uvalue_of_struct_bits := (
+        fix uvalue_of_struct_bits
+          {fields: list (string * type)} (bs: list bool)
+        : option (list val) :=
+          match fields with
+          | [] => Some []
+          | (nm, tau)::fields =>
+            let/opt2 b0, b1 := take_drop (List.length bs - type_sz tau) bs in
+            let/opt tl := uvalue_of_struct_bits (fields:=fields) b0 in
+            let/opt hd := uvalue_of_bits (tau:=tau) b1 in
+            Some (hd::tl)
+          end
+      ) in
       let uvalue_of_list_bits tau :=
-          fix uvalue_of_list_bits (l : list (list bool))
-          : option (list val)
-            :=
-              match l with
-              | [] => Some []
-              | hd::tl =>
-                let/opt hd := uvalue_of_bits (tau:=tau) hd in
-                let/opt tl := uvalue_of_list_bits tl in
-                Some (hd::tl)
-              end in
+        fix uvalue_of_list_bits (l : list (list bool)) : option (list val) :=
+          match l with
+          | [] => Some []
+          | hd::tl =>
+            let/opt hd := uvalue_of_bits (tau:=tau) hd in
+            let/opt tl := uvalue_of_list_bits tl in
+            Some (hd::tl)
+          end in
       match tau with
       | bits_t _ => Some (Bits (Datatypes.length bs) bs)
       | enum_t sig =>
@@ -460,19 +447,16 @@ Section Interp.
         let/opt lv := uvalue_of_struct_bits (fields:=struct_fields sig) bs in
         Some (Struct sig lv)
       | array_t sig =>
-        let/opt lbs := bits_splitn (array_len sig)
-                                   (type_sz (array_type sig)) bs in
+        let/opt lbs :=
+          bits_splitn (array_len sig) (type_sz (array_type sig)) bs in
         let/opt lv := uvalue_of_list_bits (array_type sig) (rev lbs) in
         Some (Array sig lv)
       end
     .
 
-
     Lemma uvalue_of_bits_val:
       forall tau v,
-        wt_val tau v ->
-        uvalue_of_bits (tau:=tau) (ubits_of_value v) =
-        Some v.
+      wt_val tau v -> uvalue_of_bits (tau:=tau) (ubits_of_value v) = Some v.
     Proof.
       intros tau v WT.
       pattern tau, v.
@@ -488,28 +472,29 @@ Section Interp.
           erewrite ubits_of_value_len'. 2: eauto.
           rewrite take_drop_head. 2: lia. simpl.
           generalize (IHstruct_fields l' H5 H7). intro A.
-          match type of A with
-            context[ let/opt _ := ?a in _ ] => destruct a eqn:?
+          match type of A with context[ let/opt _ := ?a in _ ]
+          => destruct a eqn:?
           end; simpl in *; try congruence.
           rewrite H4. simpl. inv A; auto. auto.
-      -
-        assert (Forall (fun v => wt_val (array_type sig) v /\ uvalue_of_bits (tau:= array_type sig) (ubits_of_value v) = Some v) lv).
-        {
-          rewrite Forall_forall in *; simpl; intros.
-          split; eauto.
-        }
+      - assert (Forall (
+          fun v => wt_val (array_type sig) v
+          /\ uvalue_of_bits (tau:= array_type sig) (ubits_of_value v) = Some v
+        ) lv).
+        { rewrite Forall_forall in *; simpl; intros. split; eauto. }
         clear H H0.
-
         rewrite bits_splitn_concat.
         simpl.
         rewrite rev_involutive.
-        cut ((fix uvalue_of_list_bits (l : list (list bool)) : option (list val) :=
-                match l with
-                | [] => Some []
-                | hd :: tl =>
-                  let/opt hd0 := uvalue_of_bits (tau:=array_type sig) hd
-                  in (let/opt tl0 := uvalue_of_list_bits tl in Some (hd0 :: tl0))
-                end) ((map ubits_of_value lv)) = Some lv).
+        cut (
+          (fix uvalue_of_list_bits (l : list (list bool)) : option (list val) :=
+            match l with
+            | [] => Some []
+            | hd :: tl =>
+              let/opt hd0 := uvalue_of_bits (tau:=array_type sig) hd
+              in (let/opt tl0 := uvalue_of_list_bits tl in Some (hd0 :: tl0))
+            end
+          ) ((map ubits_of_value lv)) = Some lv
+        ).
         intro A; rewrite A. simpl. reflexivity.
         revert H1 H2. generalize lv (array_len sig). clear.
         intros l n EQ. subst. revert l.
@@ -544,23 +529,19 @@ Section Interp.
         rewrite vect_to_list_length. auto.
     Qed.
 
-
     Lemma uvalue_of_bits_val':
       forall tau v,
-        uvalue_of_bits (tau:=tau) (ubits_of_value (val_of_value (tau:=tau) v)) =
-        Some (val_of_value (tau:=tau) v).
+      uvalue_of_bits (tau:=tau) (ubits_of_value (val_of_value (tau:=tau) v)) =
+      Some (val_of_value (tau:=tau) v).
     Proof.
       intros.
       apply uvalue_of_bits_val.
       apply wt_val_of_value.
     Qed.
 
-    Locate CircuitPrimSpecs.sigma1.
-
-    Compute vect_of_list [true; true; false].
-
-    Import PrimUntyped.
-    Definition usigma1' (fn: PrimUntyped.ubits1) (bs: list bool) : option (list bool) :=
+    Definition usigma1' (fn: PrimUntyped.ubits1) (bs: list bool)
+      : option (list bool)
+    :=
       match fn with
       | UNot => Some (List.map negb bs)
       | USExt w =>
@@ -580,13 +561,14 @@ Section Interp.
 
     Definition usigma1 fn v : option val :=
       match v with
-        Bits _ bs =>
-        let/opt res := usigma1' fn bs in
-        Some (Bits (List.length res) res)
+      | Bits _ bs =>
+        let/opt res := usigma1' fn bs in Some (Bits (List.length res) res)
       | _ => None
       end.
 
-    Fixpoint get_field_struct (s: list (string * type)) (lv: list val) f : option val :=
+    Fixpoint get_field_struct (s: list (string * type)) (lv: list val) f
+      : option val
+    :=
       match s, lv with
       | (n, _)::s, a::lv =>
         if eq_dec n f
@@ -595,22 +577,19 @@ Section Interp.
       | _, _ => None
       end.
 
-
-    Fixpoint find_field_offset_right (s: list (string * type)) f : option (nat * nat) :=
+    Fixpoint find_field_offset_right (s: list (string * type)) f
+      : option (nat * nat)
+    :=
       match s with
       | (n, t)::s =>
-        if eq_dec f n
-        then
-          Some (struct_fields_sz s, type_sz t)
-        else
-          find_field_offset_right s f
+        if eq_dec f n then Some (struct_fields_sz s, type_sz t)
+        else find_field_offset_right s f
       | [] => None
       end.
 
     Definition get_field (s: val) f : option val :=
       match s with
-        Struct sig lv =>
-        get_field_struct (struct_fields sig) lv f
+      | Struct sig lv => get_field_struct (struct_fields sig) lv f
       | _ => None
       end.
 
@@ -624,8 +603,7 @@ Section Interp.
       | PrimUntyped.UConv fn =>
         match fn with
         | PrimUntyped.UPack => fun v =>
-                                 let bs := ubits_of_value v in
-                                 Some (Bits (List.length bs) bs)
+          let bs := ubits_of_value v in Some (Bits (List.length bs) bs)
         | PrimUntyped.UUnpack tau =>
           fun bs =>
             match bs with
@@ -644,19 +622,20 @@ Section Interp.
       | PrimUntyped.UArray1 (PrimUntyped.UGetElement idx) =>
         fun v =>
           match v with
-          | Array sig l =>
-            List.nth_error l idx
+          | Array sig l => List.nth_error l idx
           | _ => None
           end
       | PrimUntyped.UArray1 (PrimUntyped.UGetElementBits sig idx) =>
         fun v =>
-          usigma1 (USlice (element_sz sig * (array_len sig - S idx)) (element_sz sig)) v
+          usigma1 (
+            USlice (element_sz sig * (array_len sig - S idx)) (element_sz sig)
+          ) v
       end.
-
 
     Lemma uvalue_of_bits_val_of_value:
       forall (tau: type) (v: vect bool (type_sz tau)),
-        uvalue_of_bits (tau:=tau) (vect_to_list v) = Some (val_of_value (value_of_bits v)).
+      uvalue_of_bits (tau := tau) (vect_to_list v)
+        = Some (val_of_value (value_of_bits v)).
     Proof.
       intros; rewrite <- uvalue_of_bits_val'. f_equal.
       erewrite <- ubits_of_value_ok. 2: eauto.
@@ -664,8 +643,7 @@ Section Interp.
     Qed.
 
     Lemma repeat_bits_const:
-      forall x n,
-        repeat x n = vect_to_list (Bits.const n x).
+      forall x n, repeat x n = vect_to_list (Bits.const n x).
     Proof.
       induction n; simpl; auto.
       rewrite IHn. reflexivity.
@@ -673,7 +651,7 @@ Section Interp.
 
     Lemma last_nth:
       forall {A} d (l: list A),
-        last l d = nth (List.length l - 1) l d.
+      last l d = nth (List.length l - 1) l d.
     Proof.
       induction l; simpl; intros; eauto.
       destr. simpl. auto.
@@ -682,7 +660,7 @@ Section Interp.
 
     Lemma bits_nth_list:
       forall s (v: vect bool s) idx,
-        Bits.nth v idx = nth (index_to_nat idx) (vect_to_list v) false.
+      Bits.nth v idx = nth (index_to_nat idx) (vect_to_list v) false.
     Proof.
       induction s; intros. simpl in idx; easy.
       unfold Bits.nth. destr. simpl. auto. fold @vect_nth.
@@ -691,7 +669,7 @@ Section Interp.
 
     Lemma msb_spec:
       forall s (v: bits s),
-        Bits.msb v = last (vect_to_list v) false.
+      Bits.msb v = last (vect_to_list v) false.
     Proof.
       unfold Bits.msb. intros.
       destr. destruct v. reflexivity.
@@ -704,11 +682,10 @@ Section Interp.
       apply index_of_nat_largest.
     Qed.
 
-
     Lemma vect_extend_end_firstn:
       forall x s' (v: bits (Nat.min x s')) d,
-        vect_to_list (vect_extend_end_firstn v d) =
-        vect_to_list (vect_extend_end v x d).
+      vect_to_list (vect_extend_end_firstn v d) =
+      vect_to_list (vect_extend_end v x d).
     Proof.
       unfold vect_extend_end_firstn.
       intros. rewrite vect_to_list_eq_rect. auto.
@@ -716,14 +693,14 @@ Section Interp.
 
     Lemma vect_to_list_cons:
       forall {A: Type} e s (v: vect A s),
-        vect_to_list (e::v)%vect = e:: vect_to_list v.
+      vect_to_list (e::v)%vect = e:: vect_to_list v.
     Proof.
       reflexivity.
     Qed.
 
     Lemma vect_firstn_to_list:
       forall s (v: bits s) n,
-        vect_to_list (vect_firstn n v) = fst (take_drop' n (vect_to_list v)).
+      vect_to_list (vect_firstn n v) = fst (take_drop' n (vect_to_list v)).
     Proof.
       induction s; simpl; intros. simpl in *. destruct v. destr; reflexivity.
       destr. reflexivity.
@@ -741,7 +718,7 @@ Section Interp.
 
     Lemma vect_skipn_to_list:
       forall s (v: bits s) n,
-        vect_to_list (vect_skipn n v) = snd (take_drop' n (vect_to_list v)).
+      vect_to_list (vect_skipn n v) = snd (take_drop' n (vect_to_list v)).
     Proof.
       induction s; simpl; intros. simpl in *. destruct v. destr; reflexivity.
       destr. reflexivity.
@@ -755,13 +732,13 @@ Section Interp.
 
     Lemma take_drop'_spec2:
       forall {A:Type} (n: nat) (l la lb: list A),
-        take_drop' n l = (la, lb) ->
-        l = la ++ lb /\
-        List.length la = Nat.min n (List.length l).
+      take_drop' n l = (la, lb) ->
+      l = la ++ lb /\ List.length la = Nat.min n (List.length l).
     Proof.
       induction n; simpl; intros; eauto.
       inversion H; clear H; subst. repeat split; try reflexivity.
-      destruct l; simpl in *. unfold take_drop' in H. simpl in *. inversion H; clear H.
+      destruct l; simpl in *. unfold take_drop' in H. simpl in *.
+      inversion H; clear H.
       simpl. repeat split; lia.
       destruct (take_drop' n l) as (l1 & l2) eqn:?.
       erewrite take_drop'_cons in H; eauto. inv H. simpl.
@@ -770,15 +747,13 @@ Section Interp.
     Qed.
 
     Lemma struct_fields_sz_skipn:
-      forall n f,
-        struct_fields_sz (skipn n f) <= struct_fields_sz f.
+      forall n f, struct_fields_sz (skipn n f) <= struct_fields_sz f.
     Proof.
       induction n; simpl; intros; eauto. destr. auto.
       etransitivity. apply IHn. unfold struct_fields_sz. simpl. lia.
     Qed.
     Lemma field_offset_right_le:
-      forall sig s,
-        field_offset_right sig s <= struct_sz sig.
+      forall sig s, field_offset_right sig s <= struct_sz sig.
     Proof.
       unfold field_offset_right, struct_sz.
       simpl type_sz.
@@ -787,8 +762,9 @@ Section Interp.
 
     Lemma find_field_offset_right_spec:
       forall f sig (i: index (List.length (struct_fields sig))),
-        PrimTypeInference.find_field sig f = Success i ->
-        find_field_offset_right (struct_fields sig) f = Some (field_offset_right sig i, field_sz sig i).
+      PrimTypeInference.find_field sig f = Success i ->
+      find_field_offset_right (struct_fields sig) f
+        = Some (field_offset_right sig i, field_sz sig i).
     Proof.
       intros f sig i FF.
       unfold PrimTypeInference.find_field in FF. unfold opt_result in FF.
@@ -805,14 +781,16 @@ Section Interp.
 
     Lemma usigma1_correct:
       forall ufn fn,
-        PrimTypeInference.tc1 ufn (arg1Sig (PrimSignatures.Sigma1 fn)) = Success fn ->
+      PrimTypeInference.tc1 ufn (arg1Sig (PrimSignatures.Sigma1 fn))
+        = Success fn ->
         forall (arg: arg1Sig (PrimSignatures.Sigma1 fn)) ret,
-          PrimSpecs.sigma1 fn arg = ret ->
-          sigma1 ufn (val_of_value arg) = Some (val_of_value ret).
+        PrimSpecs.sigma1 fn arg = ret ->
+        sigma1 ufn (val_of_value arg) = Some (val_of_value ret).
     Proof.
       destruct ufn; simpl; intros.
       - destruct fn.
-        + destr_in H; try congruence. inv H. simpl in *. inv Heqr. subst. reflexivity.
+        + destr_in H; try congruence. inv H. simpl in *. inv Heqr.
+          subst. reflexivity.
         + subst. inv H.
           revert arg. rewrite <- H1. simpl.
           intro arg. reflexivity.
@@ -844,9 +822,11 @@ Section Interp.
             rewrite repeat_length. rewrite vect_to_list_length. lia.
           * unfold Bits.extend_end. simpl.
             unfold eq_rect.
-            refine (match vect_extend_end_cast s width with
-                    | eq_refl => _
-                    end).
+            refine (
+              match vect_extend_end_cast s width with
+              | eq_refl => _
+              end
+            ).
             rewrite vect_to_list_app. f_equal.
             rewrite vect_to_list_length.
             rewrite repeat_bits_const. f_equal.
@@ -855,9 +835,11 @@ Section Interp.
             rewrite repeat_length. rewrite vect_to_list_length. lia.
           * unfold Bits.extend_beginning. simpl.
             unfold eq_rect.
-            refine (match vect_extend_beginning_cast s width with
-                    | eq_refl => _
-                    end).
+            refine (
+              match vect_extend_beginning_cast s width with
+              | eq_refl => _
+              end
+            ).
             rewrite vect_to_list_app. f_equal.
             rewrite vect_to_list_length.
             rewrite repeat_bits_const. f_equal.
@@ -877,7 +859,6 @@ Section Interp.
           rewrite app_length.
           rewrite repeat_length. lia.
           unfold Bits.slice.
-
           rewrite vect_extend_end_firstn.
           unfold Bits.extend_end.
           rewrite vect_to_list_eq_rect.
@@ -887,10 +868,11 @@ Section Interp.
           rewrite Heq1. simpl. rewrite Heq2. simpl.
           rewrite <- repeat_bits_const.
           f_equal. f_equal. f_equal.
-
-          apply take_drop'_spec2 in Heq2. destruct Heq2 as (Heq21 & Heq22). rewrite Heq22.
+          apply take_drop'_spec2 in Heq2. destruct Heq2 as (Heq21 & Heq22).
+          rewrite Heq22.
           apply take_drop'_spec2 in Heq1. destruct Heq1 as (Heq11 & Heq12).
-          cut (List.length l2 = s - List.length l1). intro A; rewrite A. rewrite Heq12.
+          cut (List.length l2 = s - List.length l1). intro A; rewrite A.
+          rewrite Heq12.
           rewrite vect_to_list_length. lia.
           erewrite <- (vect_to_list_length (sz:=s)). rewrite Heq11.
           rewrite app_length. lia.
@@ -914,18 +896,17 @@ Section Interp.
         + destr_in H; inv H.
           simpl PrimSpecs.sigma1.
           simpl.
-          erewrite find_field_offset_right_spec; eauto. simpl. destr. destr. simpl. f_equal.
+          erewrite find_field_offset_right_spec; eauto. simpl. destr. destr.
+          simpl. f_equal.
           unfold take_drop' in Heqp.
           edestruct (@take_drop_succeeds) as (la & lb & EQ).
           2: rewrite EQ in Heqp.
           rewrite vect_to_list_length.
-
           apply field_offset_right_le.
           f_equal.
           rewrite app_length. rewrite repeat_length.
           cut (List.length l1 <= field_sz sig s). lia.
           apply take_drop'_spec in Heqp0. intuition.
-
           unfold Bits.slice. rewrite vect_extend_end_firstn.
           unfold Bits.extend_end.
           rewrite vect_to_list_eq_rect.
@@ -952,18 +933,21 @@ Section Interp.
           unfold opt_result in Heqr. destr_in Heqr; inv Heqr.
           apply index_to_nat_of_nat in Heqo. subst.
           unfold take_drop' in *.
-          edestruct @take_drop_succeeds as (la & lb & EQ). 2: rewrite EQ in Heqp.
-          rewrite vect_to_list_length. unfold array_sz. simpl. rewrite Bits.rmul_correct.
+          edestruct @take_drop_succeeds as (la & lb & EQ).
+          2: rewrite EQ in Heqp.
+          rewrite vect_to_list_length. unfold array_sz. simpl.
+          rewrite Bits.rmul_correct.
           rewrite Nat.mul_comm. unfold element_sz. apply Nat.mul_le_mono_r.
           cut (index_to_nat s < array_len sig). lia. eapply lt_le_trans.
           apply index_to_nat_bounded. lia.
           inv Heqp.
           generalize EQ; intro EQs.
           apply take_drop_spec in EQ. intuition.
-          edestruct @take_drop_succeeds as (la & lb & EQ'). 2: rewrite EQ' in Heqp0.
-          rewrite H2, vect_to_list_length. unfold array_sz. simpl. rewrite Bits.rmul_correct.
+          edestruct @take_drop_succeeds as (la & lb & EQ').
+          2: rewrite EQ' in Heqp0.
+          rewrite H2, vect_to_list_length. unfold array_sz. simpl.
+          rewrite Bits.rmul_correct.
           unfold element_sz.
-          (* rewrite Nat.mul_comm. unfold element_sz. apply Nat.mul_le_mono_r. *)
           cut (index_to_nat s < array_len sig). nia.
           apply index_to_nat_bounded.
           f_equal. f_equal.
@@ -994,9 +978,12 @@ Section Interp.
     Definition enum_sig_eq_dec (s1 s2: enum_sig) : {s1 = s2} + {s1 <> s2}.
     Proof.
       destruct s1, s2; simpl.
-      destruct (eq_dec enum_name enum_name0). 2: right; intro A; inv A; congruence.
-      destruct (eq_dec enum_size enum_size0). 2: right; intro A; inv A; congruence.
-      destruct (eq_dec enum_bitsize enum_bitsize0). 2: right; intro A; inv A; congruence.
+      destruct (eq_dec enum_name enum_name0).
+      2: right; intro A; inv A; congruence.
+      destruct (eq_dec enum_size enum_size0).
+      2: right; intro A; inv A; congruence.
+      destruct (eq_dec enum_bitsize enum_bitsize0).
+      2: right; intro A; inv A; congruence.
       subst.
       destruct (eq_dec enum_members enum_members0).
       destruct (eq_dec enum_bitpatterns enum_bitpatterns0).
@@ -1008,18 +995,18 @@ Section Interp.
       apply Eqdep_dec.inj_pair2_eq_dec in H0. 2: apply eq_dec. congruence.
     Defined.
 
-
     Definition struct_sig_eq_dec (s1 s2: struct_sig) : {s1 = s2} + {s1 <> s2}.
     Proof.
       destruct s1, s2; simpl.
-      destruct (eq_dec struct_name struct_name0). 2: right; intro A; inv A; congruence.
-      destruct (eq_dec struct_fields struct_fields0). 2: right; intro A; inv A; congruence.
+      destruct (eq_dec struct_name struct_name0).
+      2: right; intro A; inv A; congruence.
+      destruct (eq_dec struct_fields struct_fields0).
+      2: right; intro A; inv A; congruence.
       left; subst; reflexivity.
     Defined.
 
     Lemma strong_ind_type:
-      forall (P: nat -> Type)
-             (IH: forall n, (forall m, m < n -> P m) -> P n),
+      forall (P: nat -> Type) (IH: forall n, (forall m, m < n -> P m) -> P n),
       forall n, forall m, m <= n -> P m.
     Proof.
       induction n. intros. apply IH. lia.
@@ -1030,17 +1017,16 @@ Section Interp.
     Qed.
 
     Lemma val_ind':
-      forall (P : val -> Type)
-             (Hbits: forall (n : nat) (bs : list bool), P (Bits n bs))
-             (Henum: forall (sig : enum_sig) (bs : list bool),
-                 P (Enum sig bs))
-             (Hstruct: forall (sig : struct_sig) (lv : list val),
-                 (forall x, In x lv -> P x) ->
-                 P (Struct sig lv))
-             (Harray: forall (sig : array_sig) (lv : list val),
-                 (forall x, In x lv -> P x) ->
-                 P (Array sig lv)),
-      forall (v : val), P v.
+      forall
+        (P : val -> Type)
+        (Hbits: forall (n : nat) (bs : list bool), P (Bits n bs))
+        (Henum: forall (sig : enum_sig) (bs : list bool), P (Enum sig bs))
+        (Hstruct: forall (sig : struct_sig) (lv : list val),
+          (forall x, In x lv -> P x) -> P (Struct sig lv)
+        )
+        (Harray: forall (sig : array_sig) (lv : list val),
+          (forall x, In x lv -> P x) -> P (Array sig lv)
+        ), forall (v : val), P v.
     Proof.
       intros P Hbits Henum Hstruct Harray v.
       remember (size_val v).
@@ -1048,14 +1034,9 @@ Section Interp.
       pattern n.
       eapply strong_ind_type. 2: reflexivity.
       intros n0 Plt v Heqn.
-      assert (Plt':
-                forall v,
-                  size_val v < n0 -> P v
-             ).
-      {
-        intros. eapply Plt. 2: reflexivity. lia.
-      } clear Plt.
-      rename Plt' into Plt.
+      assert (Plt': forall v, size_val v < n0 -> P v).
+      { intros. eapply Plt. 2: reflexivity. lia. }
+      clear Plt. rename Plt' into Plt.
       subst.
       destruct v; eauto.
       - eapply Hstruct.
@@ -1074,7 +1055,10 @@ Section Interp.
         eapply lt_le_trans. apply IHv; auto. lia.
     Qed.
 
-    Definition list_eq_dec' {A: Type} (l1 l2: list A) (Aeq: forall x y, In x l1 -> {x = y} + {x <> y}): {l1 = l2} + {l1 <> l2}.
+    Definition list_eq_dec'
+      {A: Type} (l1 l2: list A)
+      (Aeq: forall x y, In x l1 -> {x = y} + {x <> y})
+      : {l1 = l2} + {l1 <> l2}.
     Proof.
       revert l1 Aeq l2; induction l1; simpl; intros.
       - destruct l2. left; reflexivity. right; intro B; inv B.
@@ -1096,20 +1080,28 @@ Section Interp.
         destruct (eq_dec bs v); try (right; intro A; inv A; congruence).
         subst; left; reflexivity.
       - destruct v2; try (right; intro A; inv A; congruence).
-        destruct (enum_sig_eq_dec sig sig0); try (right; intro A; inv A; congruence).
-        destruct (eq_dec bs v); try (right; intro A; inv A; congruence).
+        destruct (enum_sig_eq_dec sig sig0);
+          try (right; intro A; inv A; congruence).
+        destruct (eq_dec bs v);
+          try (right; intro A; inv A; congruence).
         subst; left; reflexivity.
       - destruct v2; try (right; intro A; inv A; congruence).
-        destruct (struct_sig_eq_dec sig sig0); try (right; intro A; inv A; congruence).
-        destruct (list_eq_dec' lv v); try (right; intro A; inv A; congruence). eauto.
+        destruct (struct_sig_eq_dec sig sig0);
+          try (right; intro A; inv A; congruence).
+        destruct (list_eq_dec' lv v);
+          try (right; intro A; inv A; congruence). eauto.
         left; subst. reflexivity.
       - destruct v2; try (right; intro A; inv A; congruence).
-        destruct (eq_dec sig sig0); subst. 2: (right; intro A; inv A; congruence).
-        destruct (list_eq_dec' lv v); try (right; intro A; inv A; congruence). eauto.
+        destruct (eq_dec sig sig0); subst.
+        2: (right; intro A; inv A; congruence).
+        destruct (list_eq_dec' lv v);
+          try (right; intro A; inv A; congruence). eauto.
         left; subst. reflexivity.
     Defined.
 
-    Fixpoint bitwise (f: bool -> bool -> bool) (l1 l2: list bool) {struct l1}: list bool :=
+    Fixpoint bitwise (f: bool -> bool -> bool) (l1 l2: list bool) {struct l1}
+      : list bool
+    :=
       match l1, l2 with
       | [], [] => []
       | [], l2 => map (fun x => f false x) l2
@@ -1118,8 +1110,13 @@ Section Interp.
       end.
 
     Lemma and_correct:
-      forall sz (arg1: arg1Sig (PrimSignatures.Sigma2 (PrimTyped.Bits2 (PrimTyped.And sz))))
-             (arg2: arg2Sig (PrimSignatures.Sigma2 (PrimTyped.Bits2 (PrimTyped.And sz)))) ret,
+      forall sz
+        (arg1:
+          arg1Sig (PrimSignatures.Sigma2 (PrimTyped.Bits2 (PrimTyped.And sz)))
+        )
+        (arg2:
+          arg2Sig (PrimSignatures.Sigma2 (PrimTyped.Bits2 (PrimTyped.And sz)))
+        ) ret,
         PrimSpecs.sigma2 (PrimTyped.Bits2 (PrimTyped.And sz)) arg1 arg2 = ret ->
         match val_of_value arg1, val_of_value arg2 with
         | Bits _ arg1, Bits _ arg2 =>
@@ -1136,15 +1133,14 @@ Section Interp.
       reflexivity.
     Qed.
 
-
-    Lemma len_to_list: forall sz (v: bits sz), sz = Datatypes.length (vect_to_list v).
+    Lemma len_to_list:
+      forall sz (v: bits sz), sz = Datatypes.length (vect_to_list v).
     Proof.
       intros; rewrite vect_to_list_length. reflexivity.
     Defined.
 
     Lemma vect_to_list_of_list:
-      forall (v: list bool),
-        vect_to_list (vect_of_list v) = v.
+      forall (v: list bool), vect_to_list (vect_of_list v) = v.
     Proof.
       induction v; simpl; intros. reflexivity.
       rewrite vect_to_list_cons. congruence.
@@ -1152,18 +1148,16 @@ Section Interp.
 
     Lemma vect_of_list_to_list:
       forall sz (v: bits sz),
-        vect_of_list (vect_to_list v) = rew [vect bool] (len_to_list sz v) in v.
+      vect_of_list (vect_to_list v) = rew [vect bool] (len_to_list sz v) in v.
     Proof.
       intros. apply vect_to_list_inj.
       rewrite vect_to_list_of_list.
       rewrite vect_to_list_eq_rect. reflexivity.
     Qed.
 
-
     Lemma vect_to_list_vect_unsnoc:
       forall sz (v: bits (S sz)) b v',
-        vect_unsnoc v = (b, v') ->
-        vect_to_list v' = removelast (vect_to_list v).
+      vect_unsnoc v = (b, v') -> vect_to_list v' = removelast (vect_to_list v).
     Proof.
       induction sz; simpl; intros.
       - inv H. destruct v. simpl. reflexivity.
@@ -1172,11 +1166,10 @@ Section Interp.
         erewrite IHsz. 2: eauto. simpl. reflexivity.
     Qed.
 
-
     Lemma lsl1:
       forall sz (v: bits sz),
-        sz <> 0 ->
-        vect_to_list (Bits.lsl1 v) = false :: removelast (vect_to_list v).
+      sz <> 0 ->
+      vect_to_list (Bits.lsl1 v) = false :: removelast (vect_to_list v).
     Proof.
       unfold Bits.lsl1. destruct sz. congruence. intros.
       rewrite vect_to_list_cons. f_equal.
@@ -1186,13 +1179,13 @@ Section Interp.
 
     Lemma lsl1':
       forall sz (v: bits sz),
-        vect_to_list (Bits.lsl1 v) = if eq_dec sz O then [] else false :: removelast (vect_to_list v).
+      vect_to_list (Bits.lsl1 v) =
+        if eq_dec sz O then [] else false :: removelast (vect_to_list v).
     Proof.
       intros. destr.
       subst. destruct v; reflexivity.
       apply lsl1; auto.
     Qed.
-
 
     Definition ubits2_sigma (ub: ubits2) (v1 v2: list bool) : list bool :=
       match ub with
@@ -1202,19 +1195,20 @@ Section Interp.
       | ULsl =>
         let amount := Bits.to_nat (vect_of_list v2) in
         Nat.iter amount (fun v =>
-                           if eq_dec (List.length v1) O then [] else false :: removelast v) v1
+          if eq_dec (List.length v1) O then [] else false :: removelast v
+        ) v1
       | ULsr =>
         let amount := Bits.to_nat (vect_of_list v2) in
         Nat.iter amount (fun v =>
-                           if eq_dec (List.length v1) O then [] else tl v ++ [false]) v1
+          if eq_dec (List.length v1) O then [] else tl v ++ [false]
+        ) v1
       | UAsr =>
         let amount := Bits.to_nat (vect_of_list v2) in
         Nat.iter amount (fun v =>
-                           if eq_dec (List.length v1) O then [] else tl v ++ [last v false]) v1
-      | UConcat =>
-        v2 ++ v1
-      | USel =>
-        [List.nth (Bits.to_nat (vect_of_list v2)) v1 false]
+          if eq_dec (List.length v1) O then [] else tl v ++ [last v false]
+        ) v1
+      | UConcat => v2 ++ v1
+      | USel => [List.nth (Bits.to_nat (vect_of_list v2)) v1 false]
       | USliceSubst ofs w =>
         let '(h, _) := take_drop' ofs v1 in
         let '(_, t) := take_drop' (ofs + w) v1 in
@@ -1225,46 +1219,55 @@ Section Interp.
         let '(bs, _) := take_drop' w bs in
         (bs ++ List.repeat false (w - Nat.min w (List.length v1 - ofs)))
       | UPlus =>
-        vect_to_list (Bits.of_N (List.length v1) (Bits.to_N (vect_of_list v1) + Bits.to_N (vect_of_list v2)))
+        vect_to_list (
+          Bits.of_N (List.length v1) (Bits.to_N (vect_of_list v1)
+          + Bits.to_N (vect_of_list v2))
+        )
       | UMinus =>
-        vect_to_list (Bits.of_N (List.length v1)
-                                (Bits.to_N (Bits.of_N (List.length v1) (Bits.to_N (vect_of_list v1) + Bits.to_N (Bits.neg (vect_of_list v2)))) + Bits.to_N (sz:=List.length v1) Bits.one))
-
+        vect_to_list (
+          Bits.of_N (List.length v1)
+          (Bits.to_N (
+            Bits.of_N (List.length v1) (
+              Bits.to_N (vect_of_list v1)
+              + Bits.to_N (Bits.neg (vect_of_list v2))
+            )
+          ) + Bits.to_N (sz:=List.length v1) Bits.one)
+        )
       | UMul =>
-        vect_to_list (Bits.of_N (List.length v1 + List.length v2) (Bits.to_N (vect_of_list v1) * Bits.to_N (vect_of_list v2)))
+        vect_to_list (
+          Bits.of_N (List.length v1 + List.length v2)
+          (Bits.to_N (vect_of_list v1) * Bits.to_N (vect_of_list v2))
+        )
       | UCompare signed c =>
         let sz1 := List.length v1 in
         let sz2 := List.length v2 in
         match eq_dec sz2 sz1 with
         | left pf =>
           let v1 := vect_of_list v1 in
-          let v2 := rew [Bits.bits] pf in vect_of_list v2 in
-              [((if signed
-                 then
-                   match c with
-                   | cLt =>  Bits.signed_lt
-                   | cGt =>  Bits.signed_gt
-                   | cLe =>  Bits.signed_le
-                   | cGe =>  Bits.signed_ge
-                   end
-                 else
-                   match c with
-                   | cLt =>  Bits.unsigned_lt
-                   | cGt =>  Bits.unsigned_gt
-                   | cLe =>  Bits.unsigned_le
-                   | cGe =>  Bits.unsigned_ge
-                   end) v1 v2)]
+          let v2 := rew [Bits.bits] pf in vect_of_list v2 in [((
+            if signed then
+              match c with
+              | cLt => Bits.signed_lt
+              | cGt => Bits.signed_gt
+              | cLe => Bits.signed_le
+              | cGe => Bits.signed_ge
+              end
+            else
+              match c with
+              | cLt => Bits.unsigned_lt
+              | cGt => Bits.unsigned_gt
+              | cLe => Bits.unsigned_le
+              | cGe => Bits.unsigned_ge
+              end
+          ) v1 v2)]
         | _ => []
         end
-
       end.
 
-    Import PrimTyped.
-
     Lemma and_correct':
-      forall sz (arg1: bits_t sz)
-             (arg2: bits_t sz),
-        bitwise andb (vect_to_list arg1) (vect_to_list arg2) = vect_to_list (Bits.and arg1 arg2).
+      forall sz (arg1: bits_t sz) (arg2: bits_t sz),
+      bitwise andb (vect_to_list arg1) (vect_to_list arg2)
+      = vect_to_list (Bits.and arg1 arg2).
     Proof.
       induction sz; simpl. reflexivity.
       destruct arg1, arg2. simpl.
@@ -1273,11 +1276,10 @@ Section Interp.
       reflexivity.
     Qed.
 
-
     Lemma or_correct':
-      forall sz (arg1: bits_t sz)
-             (arg2: bits_t sz),
-        bitwise orb (vect_to_list arg1) (vect_to_list arg2) = vect_to_list (Bits.or arg1 arg2).
+      forall sz (arg1: bits_t sz) (arg2: bits_t sz),
+      bitwise orb (vect_to_list arg1) (vect_to_list arg2)
+      = vect_to_list (Bits.or arg1 arg2).
     Proof.
       induction sz; simpl. reflexivity.
       destruct arg1, arg2. simpl.
@@ -1286,11 +1288,10 @@ Section Interp.
       reflexivity.
     Qed.
 
-
     Lemma xor_correct':
-      forall sz (arg1: bits_t sz)
-             (arg2: bits_t sz),
-        bitwise xorb (vect_to_list arg1) (vect_to_list arg2) = vect_to_list (Bits.xor arg1 arg2).
+      forall sz (arg1: bits_t sz) (arg2: bits_t sz),
+      bitwise xorb (vect_to_list arg1) (vect_to_list arg2)
+      = vect_to_list (Bits.xor arg1 arg2).
     Proof.
       induction sz; simpl. reflexivity.
       destruct arg1, arg2. simpl.
@@ -1300,16 +1301,14 @@ Section Interp.
     Qed.
 
     Lemma iter_assoc_spec:
-      forall {A:Type} (f: A -> A) n x,
-        Nat.iter n f (f x) = f (Nat.iter n f x).
+      forall {A:Type} (f: A -> A) n x, Nat.iter n f (f x) = f (Nat.iter n f x).
     Proof.
       induction n; simpl; intros; eauto.
       rewrite IHn. auto.
     Qed.
 
     Lemma vect_dotimes_spec:
-      forall {A:Type} (f: A -> A) n x,
-        vect_dotimes f n x = Nat.iter n f x.
+      forall {A:Type} (f: A -> A) n x, vect_dotimes f n x = Nat.iter n f x.
     Proof.
       induction n; simpl; intros. auto.
       rewrite IHn, iter_assoc_spec. auto.
@@ -1317,7 +1316,7 @@ Section Interp.
 
     Lemma vect_to_list_snoc:
       forall sz (v: bits sz) x,
-        vect_to_list (vect_snoc x v) = vect_to_list v ++ [x].
+      vect_to_list (vect_snoc x v) = vect_to_list v ++ [x].
     Proof.
       induction sz; simpl; intros; eauto.
       rewrite vect_to_list_cons. f_equal.
@@ -1326,8 +1325,7 @@ Section Interp.
 
     Lemma lsr1:
       forall sz (v: bits sz),
-        sz <> 0 ->
-        vect_to_list (Bits.lsr1 v) = tl (vect_to_list v) ++ [false].
+      sz <> 0 -> vect_to_list (Bits.lsr1 v) = tl (vect_to_list v) ++ [false].
     Proof.
       unfold Bits.lsr1. intros. destr.
       rewrite vect_to_list_snoc.
@@ -1337,8 +1335,9 @@ Section Interp.
 
     Lemma asr1:
       forall sz (v: bits sz),
-        sz <> 0 ->
-        vect_to_list (Bits.asr1 v) = tl (vect_to_list v) ++ [last (vect_to_list v) false].
+      sz <> 0 ->
+        vect_to_list (Bits.asr1 v)
+        = tl (vect_to_list v) ++ [last (vect_to_list v) false].
     Proof.
       unfold Bits.asr1. intros. destr.
       rewrite vect_to_list_snoc. f_equal.
@@ -1346,10 +1345,11 @@ Section Interp.
     Qed.
 
     Lemma iter_list_vect:
-      forall sz (v: bits sz) (f: list bool -> list bool) (g: bits sz -> bits sz),
-        (forall x, f (vect_to_list x) = vect_to_list (g x)) ->
+      forall sz (v: bits sz) (f: list bool -> list bool)
+        (g: bits sz -> bits sz),
+      (forall x, f (vect_to_list x) = vect_to_list (g x)) ->
         forall n,
-          Nat.iter n f (vect_to_list v) = vect_to_list (vect_dotimes g n v).
+        Nat.iter n f (vect_to_list v) = vect_to_list (vect_dotimes g n v).
     Proof.
       intros. rewrite vect_dotimes_spec. induction n; simpl; intros; eauto.
       rewrite IHn. apply H.
@@ -1357,8 +1357,8 @@ Section Interp.
 
     Lemma sel:
       forall sz (bs: bits sz) idx,
-        vect_to_list (BitFuns.sel bs idx) =
-        [List.nth (Bits.to_nat idx) (vect_to_list bs) false].
+      vect_to_list (BitFuns.sel bs idx) =
+      [List.nth (Bits.to_nat idx) (vect_to_list bs) false].
     Proof.
       unfold BitFuns.sel. intros.
       destr.
@@ -1369,12 +1369,13 @@ Section Interp.
       rewrite vect_to_list_length.
       apply index_of_nat_none_ge in Heqo. lia.
     Qed.
+
     Lemma slice_subst:
       forall sz (bs: bits sz) ofs w v,
-        vect_to_list (Bits.slice_subst ofs w bs v) =
-        let '(h, _) := take_drop' ofs (vect_to_list bs) in
-        let '(_, t) := take_drop' (ofs + w) (vect_to_list bs) in
-        fst (take_drop' sz (h ++ (vect_to_list v) ++ t)).
+      vect_to_list (Bits.slice_subst ofs w bs v) =
+      let '(h, _) := take_drop' ofs (vect_to_list bs) in
+      let '(_, t) := take_drop' (ofs + w) (vect_to_list bs) in
+      fst (take_drop' sz (h ++ (vect_to_list v) ++ t)).
     Proof.
       unfold Bits.slice_subst. intros.
       destr. destr.
@@ -1388,10 +1389,10 @@ Section Interp.
 
     Lemma slice:
       forall sz (bs: bits sz) ofs w,
-        vect_to_list (Bits.slice ofs w bs) =
-        let '(_, bs) := take_drop' ofs (vect_to_list bs) in
-        let '(bs, _) := take_drop' w bs in
-        (bs ++ List.repeat false (w - Nat.min w (sz - ofs))).
+      vect_to_list (Bits.slice ofs w bs) =
+      let '(_, bs) := take_drop' ofs (vect_to_list bs) in
+      let '(bs, _) := take_drop' w bs in
+      (bs ++ List.repeat false (w - Nat.min w (sz - ofs))).
     Proof.
       intros. unfold Bits.slice. rewrite vect_extend_end_firstn.
       unfold Bits.extend_end.
@@ -1403,40 +1404,42 @@ Section Interp.
       destr. simpl. destr. simpl.
       f_equal.
     Qed.
+
     Lemma vect_to_list_eq:
       forall sz1 sz2 (v1: bits sz1) (v2: bits sz2) (pf: sz1 = sz2),
-        rew [fun x => bits x] pf in v1 = v2 ->
-                                    vect_to_list v1 = vect_to_list v2.
+      rew [fun x => bits x] pf in v1 = v2 -> vect_to_list v1 = vect_to_list v2.
     Proof.
       intros. subst. rewrite vect_to_list_eq_rect. auto.
     Qed.
 
     Lemma bits_map_rew:
       forall sz1 sz2 (v: bits sz1) f (pf: sz1 = sz2),
-        Bits.map f (rew [Bits.bits] pf in v) = rew [Bits.bits] pf in (Bits.map f v).
+      Bits.map f (rew [Bits.bits] pf in v)
+        = rew [Bits.bits] pf in (Bits.map f v).
     Proof.
       intros. subst. simpl. auto.
     Qed.
 
     Lemma cmp:
       forall sz (v1 v2: bits sz) c,
-        vect_to_list (BitFuns.bitfun_of_predicate c v1 v2) =
-        [c v1 v2].
+      vect_to_list (BitFuns.bitfun_of_predicate c v1 v2) = [c v1 v2].
     Proof.
       unfold BitFuns.bitfun_of_predicate. simpl; intros. reflexivity.
     Qed.
+
     Lemma lift_comparison_rew:
-      forall {A} sz1 sz1' (pf: sz1 = sz1') (pf2: sz1 = sz1') (v1: bits sz1) (v2: bits sz1) (cast: forall sz, bits sz -> A) compare cmp,
-        Bits.lift_comparison (cast sz1') compare cmp (rew [Bits.bits] pf in v1) (rew [Bits.bits] pf2 in v2) =
-        Bits.lift_comparison (cast sz1) compare cmp v1 v2.
+      forall {A} sz1 sz1' (pf: sz1 = sz1') (pf2: sz1 = sz1') (v1: bits sz1)
+        (v2: bits sz1) (cast: forall sz, bits sz -> A) compare cmp,
+      Bits.lift_comparison (cast sz1') compare cmp (rew [Bits.bits] pf in v1)
+        (rew [Bits.bits] pf2 in v2)
+      = Bits.lift_comparison (cast sz1) compare cmp v1 v2.
     Proof.
       intros. subst. simpl.
       rewrite (Eqdep_dec.UIP_refl_nat _ pf2). simpl. reflexivity.
     Qed.
 
     Lemma ubits2_correct:
-      forall
-        ub b sz1 sz2
+      forall ub b sz1 sz2
         (UB:
            match ub with
            | USel => Sel sz1
@@ -1453,8 +1456,8 @@ Section Interp.
            | UMinus => Minus sz1
            | UMul => Mul sz1 sz2
            | UCompare signed c => Compare signed c sz1
-           end = b)
-        (arg1: arg1Sig (PrimSignatures.Sigma2 (PrimTyped.Bits2 b)))
+           end = b
+        ) (arg1: arg1Sig (PrimSignatures.Sigma2 (PrimTyped.Bits2 b)))
         (arg2: arg2Sig (PrimSignatures.Sigma2 (PrimTyped.Bits2 b))) ret,
         CircuitPrimSpecs.sigma2 b arg1 arg2 = ret ->
         match val_of_value arg1, val_of_value arg2 with
@@ -1484,20 +1487,22 @@ Section Interp.
         intros. rewrite vect_to_list_length. destr. subst. reflexivity.
         rewrite asr1; auto.
       - rewrite vect_to_list_app; auto.
-      - rewrite sel.
-        rewrite vect_of_list_to_list. unfold Bits.to_nat; rewrite Bits.to_N_rew. auto.
+      - rewrite sel. rewrite vect_of_list_to_list.
+        unfold Bits.to_nat; rewrite Bits.to_N_rew. auto.
       - rewrite vect_to_list_length.
         rewrite slice_subst. reflexivity.
       - rewrite slice.
         rewrite vect_of_list_to_list. unfold Bits.to_nat; rewrite Bits.to_N_rew.
-        destr. destr. f_equal. f_equal. rewrite vect_to_list_length. reflexivity.
+        destr. destr. f_equal. f_equal. rewrite vect_to_list_length.
+        reflexivity.
       - unfold Bits.plus.
         rewrite ! vect_of_list_to_list.
         rewrite ! Bits.to_N_rew.
         eapply vect_to_list_eq.
-        erewrite (f_equal_dep _ (fun x => Bits.of_N x (Bits.to_N arg1 + Bits.to_N arg2))).
-        Unshelve. 2: apply vect_to_list_length.
-        auto.
+        erewrite (f_equal_dep _ (fun x => Bits.of_N x (
+          Bits.to_N arg1 + Bits.to_N arg2
+        ))).
+        Unshelve. 2: apply vect_to_list_length. auto.
       - unfold Bits.minus.
         rewrite ! vect_of_list_to_list.
         rewrite ! Bits.to_N_rew.
@@ -1522,62 +1527,35 @@ Section Interp.
         rewrite ! vect_of_list_to_list.
         rewrite ! Bits.to_N_rew.
         eapply vect_to_list_eq.
-        erewrite (f_equal_dep _ (fun x => Bits.of_N x (Bits.to_N arg1 * Bits.to_N arg2))).
-        Unshelve. 2: rewrite ! vect_to_list_length; auto.
-        auto.
+        erewrite (f_equal_dep _ (fun x => Bits.of_N x (
+          Bits.to_N arg1 * Bits.to_N arg2
+        ))).
+        Unshelve. 2: rewrite ! vect_to_list_length; auto. auto.
       - destr.
         + rewrite ! vect_of_list_to_list.
           rewrite rew_compose.
-          transitivity ( vect_to_list
-                           (BitFuns.bitfun_of_predicate (if signed
-                                                         then
-                                                           match c with
-                                                           | cLt =>  Bits.signed_lt
-                                                           | cGt =>  Bits.signed_gt
-                                                           | cLe =>  Bits.signed_le
-                                                           | cGe =>  Bits.signed_ge
-                                                           end
-                                                         else
-                                                           match c with
-                                                           | cLt =>  Bits.unsigned_lt
-                                                           | cGt =>  Bits.unsigned_gt
-                                                           | cLe =>  Bits.unsigned_le
-                                                           | cGe =>  Bits.unsigned_ge
-                                                           end) arg1 arg2)
-                       ). 2: repeat destr; reflexivity.
+          transitivity (vect_to_list (BitFuns.bitfun_of_predicate (
+            if signed then
+              match c with
+              | cLt =>  Bits.signed_lt
+              | cGt =>  Bits.signed_gt
+              | cLe =>  Bits.signed_le
+              | cGe =>  Bits.signed_ge
+              end
+            else
+              match c with
+              | cLt =>  Bits.unsigned_lt
+              | cGt =>  Bits.unsigned_gt
+              | cLe =>  Bits.unsigned_le
+              | cGe =>  Bits.unsigned_ge
+              end
+          ) arg1 arg2)).
+          2: repeat destr; reflexivity.
           rewrite cmp. f_equal.
           repeat destr; apply lift_comparison_rew.
         + clear -n. exfalso.
           rewrite ! vect_to_list_length in n. congruence.
     Qed.
-
-
-    (*   Definition sigma2 (fn: PrimTyped.fbits2) : CSig_denote (CircuitSignatures.CSigma2 fn) := *)
-    (*     match fn with *)
-    (*     | Sel _ => sel *)
-    (*     | SliceSubst _ offset width => Bits.slice_subst offset width *)
-    (*     | IndexedSlice _ width => fun bs offset => Bits.slice (Bits.to_nat offset) width bs *)
-    (*     | And _ => Bits.and *)
-    (*     | Or _ => Bits.or *)
-    (*     | Xor _ => Bits.xor *)
-    (*     | Lsl _ _ => lsl *)
-    (*     | Lsr _ _ => lsr *)
-    (*     | Asr _ _ => asr *)
-    (*     | Concat _ _ => Bits.app *)
-    (*     | Plus _ => Bits.plus *)
-    (*     | Minus _ => Bits.minus *)
-    (*     | Mul _ _ => Bits.mul *)
-    (*     | EqBits _ false => _eq *)
-    (*     | EqBits _ true => _neq *)
-    (*     | Compare true cLt _ => bitfun_of_predicate Bits.signed_lt *)
-    (*     | Compare true cGt _ => bitfun_of_predicate Bits.signed_gt *)
-    (*     | Compare true cLe _ => bitfun_of_predicate Bits.signed_le *)
-    (*     | Compare true cGe _ => bitfun_of_predicate Bits.signed_ge *)
-    (*     | Compare false cLt _ => bitfun_of_predicate Bits.unsigned_lt *)
-    (*     | Compare false cGt _ => bitfun_of_predicate Bits.unsigned_gt *)
-    (*     | Compare false cLe _ => bitfun_of_predicate Bits.unsigned_le *)
-    (*     | Compare false cGe _ => bitfun_of_predicate Bits.unsigned_ge *)
-    (*     end. *)
 
     Fixpoint subst_field (n: nat) (v: val) (s: list val) : option (list val) :=
       match n, s with
@@ -1587,13 +1565,15 @@ Section Interp.
       end.
 
     Fixpoint val_of_struct_value'
-             (fields : list (string * type))
-             (x : struct_denote fields)
-             {struct fields} : list val :=
+      (fields : list (string * type)) (x : struct_denote fields) {struct fields}
+      : list val
+    :=
       match fields as fields0 return (struct_denote fields0 -> list val) with
       | [] => fun _ : unit => []
       | p :: fields0 =>
-        let (_, tau) as p0 return (snd p0 * struct_denote fields0 -> list val) := p in
+        let (_, tau)
+          as p0 return (snd p0 * struct_denote fields0 -> list val)
+          := p in
         fun '(x0, xs) => val_of_value x0 :: val_of_struct_value' fields0 xs
       end x.
 
